cogent/examples/wa_connect/WordArray_CorresProof_Asm.thy
@@ -11,7 +11,7 @@ context WordArray begin
 section "Level 0 Assumptions"
 
 lemma value_sem_rename_mono_prog_rename_\<Xi>_\<xi>m_\<xi>p: 
-  "value_sem.rename_mono_prog abs_typing_v rename \<Xi> \<xi>m \<xi>p"
+  "value_sem.rename_mono_prog wa_abs_typing_v rename \<Xi> \<xi>m \<xi>p"
   apply (clarsimp simp: val.rename_mono_prog_def)
   apply (rule conjI; clarsimp)
    apply (rule_tac x = v' in exI)
@@ -49,8 +49,7 @@ lemma val_proc_env_matches_\<xi>m_\<Xi>:
     apply (rule val.v_t_prim')
     apply (erule val.v_t_recordE; clarsimp)
     apply (erule val.v_t_r_consE; clarsimp)+
-    apply (erule val.v_t_abstractE; clarsimp simp: abs_typing_v_def)
-    apply (case_tac va; clarsimp)
+    apply (erule val.v_t_abstractE; clarsimp simp: wa_abs_typing_v_def)
    apply (clarsimp simp: wordarray_length_0_type_def val_wa_length_def)
    apply (rule val.v_t_prim'; clarsimp)
   apply (clarsimp simp: wordarray_put2_0_type_def abbreviatedType2_def val_wa_put2_def)
@@ -58,12 +57,12 @@ lemma val_proc_env_matches_\<xi>m_\<Xi>:
   apply (erule val.v_t_r_consE; clarsimp)
   apply (erule val.v_t_abstractE)
   apply (rule val.v_t_abstract; clarsimp)
-  apply (clarsimp simp: abs_typing_v_def)
+  apply (clarsimp simp: wa_abs_typing_v_def)
   apply (case_tac val; clarsimp)
    apply (erule_tac x = i in allE; clarsimp)
-   apply (case_tac "i = unat idx")
-    apply (rule_tac x = x4 in exI; simp)
-   apply (rule_tac x = x in exI; simp)
+  apply (case_tac "i = unat idx")
+   apply clarsimp
+  apply (rule_tac x = x in exI; simp)
   done
 
 lemma wordarray_get_upd_val:
@@ -84,21 +83,22 @@ lemma wordarray_get_upd_val:
   apply (rule conjI)
    apply (clarsimp simp: val_wa_get_def)
    apply (rule_tac x = "{}" in exI)+
-   apply (clarsimp simp: abs_upd_val'_def frame_def word_less_nat_alt)
+   apply (clarsimp simp: wa_abs_upd_val_def frame_def word_less_nat_alt)
    apply (case_tac va; clarsimp simp: word_less_nat_alt)
-   apply (erule_tac x = idx in allE)
-   apply clarsimp
+   apply (clarsimp simp: wa_abs_typing_v_def)
+   apply (case_tac v; clarsimp)
+   apply (erule_tac x = idx in allE)+
    apply (case_tac "unat idx < length xs"; clarsimp)
-    apply (rule u_v_prim'; clarsimp)
+    apply (rule u_v_prim'; clarsimp simp: word_less_nat_alt)
    apply (rule u_v_prim'; clarsimp)
-  apply (clarsimp simp: word_less_nat_alt abs_upd_val'_def)
+  apply (clarsimp simp: word_less_nat_alt wa_abs_upd_val_def)
   apply (case_tac a'; clarsimp)
   apply (case_tac x11; clarsimp)
   apply (case_tac x5; clarsimp)
-  apply (case_tac x1; clarsimp)
+  apply (case_tac x1; clarsimp simp: wa_abs_typing_v_def)
   apply (erule_tac x = idx in allE)
-  apply (case_tac "unat idx < length x12"; clarsimp  simp: word_less_nat_alt)
-   apply (rule_tac x = "VPrim (LU32 x)" in exI)
+  apply (case_tac "unat idx < length x12"; clarsimp simp: word_less_nat_alt)
+   apply (rule_tac x = "VPrim va" in exI)
    apply (clarsimp simp: val_wa_get_def)
   apply (rule_tac x = "VPrim (LU32 0)" in exI)
   apply (clarsimp simp: val_wa_get_def)
@@ -112,19 +112,22 @@ lemma wordarray_length_upd_val:
           frame \<sigma> w \<sigma>' w')) \<and> Ex (val_wa_length a')"
   apply (clarsimp simp: upd_wa_length_0_def wordarray_length_0_type_def)
   apply (erule u_v_p_absE'; clarsimp)
-  apply (clarsimp simp: abs_upd_val'_def)
+  apply (clarsimp simp: wa_abs_upd_val_def)
   apply (case_tac a'a; clarsimp)
   apply (case_tac x11; clarsimp)
   apply (case_tac x5; clarsimp)
-  apply (case_tac x1; clarsimp)
   apply (rule conjI)
    apply (clarsimp simp: val_wa_length_def)
    apply (rule_tac x = "{}" in exI)+
-   apply (clarsimp simp: frame_def intro!: u_v_prim[where l = "(LU32 _)", simplified])
-  apply (clarsimp simp: abs_upd_val'_def)
+   apply (clarsimp simp: frame_def)
+   apply (rule u_v_prim'; clarsimp)
+  apply (clarsimp simp: wa_abs_upd_val_def)
   apply (rule_tac x = "VPrim (LU32 len)" in exI)
   apply (clarsimp simp: val_wa_length_def)
   done
+
+inductive_cases u_v_t_prim_tE : "upd_val_rel \<Xi>' \<sigma> u v (TPrim l) r w"
+
 
 lemma wordarray_put2_upd_val:
   "\<And>K a b \<sigma> \<sigma>' \<tau>s aa a' v v' r w.
@@ -156,12 +159,16 @@ lemma wordarray_put2_upd_val:
    apply (rule conjI)
     apply (rule_tac a = a and  ptrl = undefined in u_v_p_abs_w[where ts = "[TPrim (Num U32)]", simplified])
        apply simp
-      apply (clarsimp simp: abs_upd_val'_def)
+      apply (clarsimp simp: wa_abs_upd_val_def)
       apply (case_tac a; clarsimp)
+      apply (case_tac x11; clarsimp)
+      apply (case_tac x5; clarsimp)
+      apply (erule u_v_t_prim_tE)
+      apply clarsimp
       apply (rule conjI)
-       apply (clarsimp simp: abs_typing_u_def)
+       apply (clarsimp simp: wa_abs_typing_u_def)
       apply (rule conjI)
-       apply (clarsimp simp: abs_typing_v_def word_less_nat_alt)
+       apply (clarsimp simp: wa_abs_typing_v_def word_less_nat_alt)
        apply (erule_tac x = i in allE)
        apply (case_tac "i = unat idx"; clarsimp)
       apply (clarsimp simp: word_less_nat_alt)
@@ -175,26 +182,35 @@ lemma wordarray_put2_upd_val:
       apply clarsimp
       apply (erule_tac x = i in allE)
       apply clarsimp
-      apply (case_tac "unat i = unat idx"; clarsimp)
-     apply (clarsimp simp: abs_upd_val'_def)
+      apply (case_tac "unat i = unat idx"; clarsimp simp: wa_abs_typing_u_def)
+     apply (clarsimp simp: wa_abs_upd_val_def)
      apply (erule_tac x = idx in allE)
      apply clarsimp
+     apply (erule u_v_t_prim_tE; simp)
     apply simp
-   apply (clarsimp simp: frame_def abs_upd_val'_def abs_typing_u_def)
-  apply (case_tac a; clarsimp)
+   apply (clarsimp simp: frame_def wa_abs_upd_val_def wa_abs_typing_u_def)
+   apply (case_tac a; clarsimp)
+   apply (case_tac x11; clarsimp)
+   apply (case_tac x5; clarsimp)
    apply (rule conjI; clarsimp)
     apply (rule conjI)
      apply clarsimp
     apply (rule conjI; clarsimp)
    apply (rule conjI; clarsimp)
-  apply (clarsimp simp: abs_upd_val'_def)
-  apply (case_tac a; clarsimp simp: abs_typing_u_def)
-  apply (case_tac a'; clarsimp)
-  apply (case_tac x11a; clarsimp)
+  apply (erule u_v_t_prim_tE; clarsimp)
+  apply (clarsimp simp: wa_abs_upd_val_def)
+  apply (case_tac a; clarsimp simp: wa_abs_typing_u_def)
+  apply (case_tac x11; clarsimp)
   apply (case_tac x5; clarsimp)
-  apply (case_tac x1; clarsimp)
-  apply (rule_tac x = "VAbstract (VWA (TPrim (Num U32)) (x12a[unat idx := VPrim (LU32 val)]))" in exI)
+  apply (case_tac a'; clarsimp)
+  apply (case_tac x11; clarsimp)
+  apply (case_tac x5; clarsimp)
+  apply (case_tac x1; clarsimp simp: wa_abs_typing_v_def)
+  apply (erule u_v_t_prim_tE; clarsimp)
+  apply (rule_tac x = "VAbstract (VWA (TPrim (Num U32)) (x12a[unat idx := VPrim l]))" in exI)
   apply (clarsimp simp: val_wa_put2_def)
+  apply (drule_tac t = "lit_type l" in sym)
+  apply clarsimp
   done
 
 lemma proc_env_u_v_matches_\<xi>0_\<xi>m_\<Xi>:
@@ -221,9 +237,9 @@ lemma wordarray_get_uval_typing_frame:
   apply (erule upd.u_t_r_emptyE; clarsimp)
   apply (erule upd.u_t_primE; subst (asm) lit_type.simps; clarsimp)+
   apply (rule_tac x = "{}" in exI)+
-  apply (clarsimp simp: frame_def abs_typing_u_def)
+  apply (clarsimp simp: frame_def wa_abs_typing_u_def)
   apply (erule_tac x = idx in allE)
-  apply (case_tac "idx < len"; clarsimp intro!: upd.u_t_prim[where l = "(LU32 _)", simplified])
+  apply (rule upd.u_t_prim'; clarsimp)
   done
 
 lemma wordarray_length_uval_typing_frame:
@@ -234,8 +250,10 @@ lemma wordarray_length_uval_typing_frame:
   apply (clarsimp simp: wordarray_length_0_type_def upd_wa_length_0_def)
   apply (erule upd.u_t_p_absE; clarsimp)
   apply (rule_tac x = "{}" in exI)+
-  apply (clarsimp simp: frame_def intro!: upd.u_t_prim[where l = "(LU32 _)", simplified])
+  apply (clarsimp simp: frame_def intro!: upd.u_t_prim')
   done
+
+inductive_cases upd_u_t_prim_tE: "upd.uval_typing \<Xi>' \<sigma> u (TPrim l) r w"
 
 lemma wordarray_put2_uval_typing_frame:
   "\<And>K a b \<sigma> \<sigma>' \<tau>s v v' r w.
@@ -262,19 +280,23 @@ lemma wordarray_put2_uval_typing_frame:
    apply (rule_tac x = ra in exI)
    apply (rule_tac x = "insert p w" in exI)
    apply (rule conjI)
-    apply (rename_tac len arr)
-    apply (rule_tac ptrl = undefined and a = "WAU32 len arr" in upd.u_t_p_abs_w[where ts = "[TPrim (Num U32)]", simplified])
+    apply (rename_tac t len arr)
+    apply (rule_tac ptrl = undefined and a = "UWA t len arr" in upd.u_t_p_abs_w[where ts = "[TPrim (Num U32)]", simplified])
        apply simp
-      apply (clarsimp simp: abs_typing_u_def)
-     apply (clarsimp simp: abs_typing_u_def)
+      apply (clarsimp simp: wa_abs_typing_u_def)
+      apply (case_tac t; clarsimp)
+      apply (case_tac x5; clarsimp)
+      apply (erule upd_u_t_prim_tE; clarsimp)
+     apply (clarsimp simp: wa_abs_typing_u_def)
     apply clarsimp
-   apply (clarsimp simp: frame_def abs_typing_u_def)
+   apply (clarsimp simp: frame_def wa_abs_typing_u_def)
    apply (rule conjI; clarsimp)
     apply (rule conjI)
      apply clarsimp
     apply (rule conjI; clarsimp)
+   apply (erule upd_u_t_prim_tE; clarsimp)
    apply (rule conjI; clarsimp)
-  apply (clarsimp simp: abs_typing_u_def)
+  apply (clarsimp simp: wa_abs_typing_u_def)
   done
 
 lemma upd_proc_env_matches_ptrs_\<xi>0_\<Xi>:
@@ -348,7 +370,7 @@ lemma wordarray_fold_no_break_uval_typing_frame:
   apply (rule upd.u_t_prim[where l = "LU32 _", simplified])
   done
 
-inductive_cases v_t_prim_tE : "val.vval_typing \<Xi>' v (TPrim (Num U32))"
+inductive_cases v_t_prim_tE : "val.vval_typing \<Xi>' v (TPrim l)"
 
 lemma lit_type_ex_32:
   "lit_type l = Num U32 \<Longrightarrow> \<exists>v. l = LU32 v"
@@ -359,44 +381,46 @@ lemma val_wa_foldnb_0_mono_helper1:
   "\<lbrakk>val.proc_env_matches \<xi>m1 \<Xi>; proc_ctx_wellformed \<Xi>; \<forall>i<length xs. \<exists>v. xs ! i = VPrim (LU32 v);
     \<Xi>, [], [option.Some Generated_TypeProof.abbreviatedType1] \<turnstile> App (Fun (val.rename_expr rename 
       (val.monoexpr (specialise ts f))) []) (Var 0) : TPrim (Num U32);
-    val_wa_foldnb_bod_0 xs frm to (Fun (val.rename_expr rename (val.monoexpr (specialise ts f))) [])
+    val_wa_foldnb_bod_0 \<xi>m xs frm to (Fun (val.rename_expr rename (val.monoexpr (specialise ts f))) [])
          (VPrim (LU32 acc)) VUnit (VPrim (LU32 r))\<rbrakk>
-       \<Longrightarrow> val_wa_foldnb_bod_0p xs frm to (Fun f ts) (VPrim (LU32 acc)) VUnit (VPrim (LU32 r))"
+       \<Longrightarrow> val_wa_foldnb_bod_0 \<xi>p xs frm to (Fun f ts) (VPrim (LU32 acc)) VUnit (VPrim (LU32 r))"
   apply (induct to arbitrary: r)
    apply (erule val_wa_foldnb_bod_0.elims; clarsimp)
-   apply (subst val_wa_foldnb_bod_0p.simps; clarsimp)
+   apply (subst val_wa_foldnb_bod_0.simps; clarsimp)
   apply clarsimp
   apply (case_tac "length xs < Suc to")
    apply (erule_tac x = r in meta_allE)
    apply (drule val_wa_foldnb_bod_0_back_step'; simp)
-   apply (drule val_wa_foldnb_bod_0p_to_geq_lenD)
+   apply (drule val_wa_foldnb_bod_0_to_geq_lenD)
     apply linarith
-   apply (rule val_wa_foldnb_bod_0p_to_geq_len; simp)
+   apply (rule val_wa_foldnb_bod_0_to_geq_len; simp)
   apply (clarsimp simp: not_less)
   apply (case_tac "frm \<ge> to")
    apply (erule val_wa_foldnb_bod_0.elims; clarsimp split: if_splits)
     apply (erule val_wa_foldnb_bod_0.elims; clarsimp)
-    apply (subst val_wa_foldnb_bod_0p.simps; clarsimp)
-    apply (subst val_wa_foldnb_bod_0p.simps; clarsimp)
-    apply (drule_tac \<gamma> = "[VRecord [VPrim (LU32 v), VPrim (LU32 acc), VUnit]]" and
+    apply (subst val_wa_foldnb_bod_0.simps; clarsimp)
+    apply (subst val_wa_foldnb_bod_0.simps; clarsimp)
+    apply (drule_tac \<gamma> = "[VRecord [xs ! frm, VPrim (LU32 acc), VUnit]]" and
       \<Gamma> = "[option.Some abbreviatedType1]" and
       e = "App (Fun f ts) (Var 0)" and
       v' = "VPrim (LU32 r)" and
       \<tau>  = "TPrim (Num U32)" in val.rename_monoexpr_correct(1)
       [OF _ val_proc_env_matches_\<xi>m_\<Xi> value_sem_rename_mono_prog_rename_\<Xi>_\<xi>m_\<xi>p]; clarsimp?)
-     apply (clarsimp simp: abbreviatedType1_def)
-     apply (clarsimp simp: val.matches_Cons[where xs = "[]" and ys = "[]", simplified])
-     apply (clarsimp simp: val.matches_def)
-     apply (rule val.v_t_record; simp?)
-     apply (rule val.v_t_r_cons1; clarsimp?)
-      apply (rule val.v_t_prim'; clarsimp)
-     apply (rule val.v_t_r_cons1; clarsimp?)
-      apply (rule val.v_t_prim'; clarsimp)
-     apply (rule val.v_t_r_cons1; clarsimp?)
-      apply (rule val.v_t_unit)
-     apply (rule val.v_t_r_empty)
-    apply (case_tac va; clarsimp)
-   apply (subst val_wa_foldnb_bod_0p.simps; clarsimp)
+      apply (clarsimp simp: abbreviatedType1_def)
+      apply (clarsimp simp: val.matches_Cons[where xs = "[]" and ys = "[]", simplified])
+      apply (clarsimp simp: val.matches_def)
+      apply (rule val.v_t_record; simp?)
+      apply (rule val.v_t_r_cons1; clarsimp?)
+       apply (erule_tac x = frm in allE; clarsimp)
+       apply (rule val.v_t_prim'; clarsimp)
+      apply (rule val.v_t_r_cons1; clarsimp?)
+       apply (rule val.v_t_prim'; clarsimp)
+      apply (rule val.v_t_r_cons1; clarsimp?)
+       apply (rule val.v_t_unit)
+      apply (rule val.v_t_r_empty)
+     apply (erule_tac x = frm in allE; clarsimp)
+    apply (case_tac v; clarsimp)
+   apply (subst val_wa_foldnb_bod_0.simps; clarsimp)
   apply (clarsimp simp: not_le)
   apply (frule_tac x = to in spec)
   apply (erule impE, simp)
@@ -424,11 +448,14 @@ lemma val_wa_foldnb_0_mono_helper1:
      apply (rule val.v_t_unit)
     apply (rule val.v_t_r_empty)
    apply (case_tac va; clarsimp)
-   apply (drule_tac v = v and r' = "VPrim (LU32 r)" in val_wa_foldnb_bod_0p_step; simp)
+   apply (drule_tac r' = "VPrim (LU32 r)" in val_wa_foldnb_bod_0_step; simp)
   apply (insert val_proc_env_matches_\<xi>m_\<Xi>)
   apply (clarsimp simp: abbreviatedType1_def)
   apply (drule val_wa_foldnb_bod_0_preservation; simp?)
-    apply (rule val.v_t_prim[where l = "LU32 _", simplified])
+     apply clarsimp
+     apply (erule_tac x = i in allE; clarsimp)
+     apply (rule val.v_t_prim'; clarsimp)
+    apply (rule val.v_t_prim'; clarsimp)
    apply (rule val.v_t_unit)
   apply (erule v_t_prim_tE)
   apply (drule lit_type_ex_32[OF sym])
@@ -439,44 +466,46 @@ lemma val_wa_foldnb_0_mono_helper2:
   "\<lbrakk>val.proc_env_matches \<xi>m1 \<Xi>; proc_ctx_wellformed \<Xi>; \<forall>i<length xs. \<exists>v. xs ! i = VPrim (LU32 v);
     \<Xi>, [], [option.Some Generated_TypeProof.abbreviatedType1] \<turnstile> App (AFun (rename (f, ts)) []) 
       (Var 0) : TPrim (Num U32);
-    val_wa_foldnb_bod_0 xs frm to (AFun (rename (f, ts)) [])
+    val_wa_foldnb_bod_0 \<xi>m xs frm to (AFun (rename (f, ts)) [])
          (VPrim (LU32 acc)) VUnit (VPrim (LU32 r))\<rbrakk>
-       \<Longrightarrow> val_wa_foldnb_bod_0p xs frm to (AFun f ts) (VPrim (LU32 acc)) VUnit (VPrim (LU32 r))"
+       \<Longrightarrow> val_wa_foldnb_bod_0 \<xi>p xs frm to (AFun f ts) (VPrim (LU32 acc)) VUnit (VPrim (LU32 r))"
   apply (induct to arbitrary: r)
    apply (erule val_wa_foldnb_bod_0.elims; clarsimp)
-   apply (subst val_wa_foldnb_bod_0p.simps; clarsimp)
+   apply (subst val_wa_foldnb_bod_0.simps; clarsimp)
   apply clarsimp
   apply (case_tac "length xs < Suc to")
    apply (erule_tac x = r in meta_allE)
    apply (drule val_wa_foldnb_bod_0_back_step'; simp)
-   apply (drule val_wa_foldnb_bod_0p_to_geq_lenD)
+   apply (drule val_wa_foldnb_bod_0_to_geq_lenD)
     apply linarith
-   apply (rule val_wa_foldnb_bod_0p_to_geq_len; simp)
+   apply (rule val_wa_foldnb_bod_0_to_geq_len; simp)
   apply (clarsimp simp: not_less)
   apply (case_tac "frm \<ge> to")
    apply (erule val_wa_foldnb_bod_0.elims; clarsimp split: if_splits)
     apply (erule val_wa_foldnb_bod_0.elims; clarsimp)
-    apply (subst val_wa_foldnb_bod_0p.simps; clarsimp)
-    apply (subst val_wa_foldnb_bod_0p.simps; clarsimp)
-    apply (drule_tac \<gamma> = "[VRecord [VPrim (LU32 v), VPrim (LU32 acc), VUnit]]" and
+    apply (subst val_wa_foldnb_bod_0.simps; clarsimp)
+    apply (subst val_wa_foldnb_bod_0.simps; clarsimp)
+    apply (drule_tac \<gamma> = "[VRecord [xs ! frm, VPrim (LU32 acc), VUnit]]" and
       \<Gamma> = "[option.Some abbreviatedType1]" and
       e = "App (AFun f ts) (Var 0)" and
       v' = "VPrim (LU32 r)" and
       \<tau>  = "TPrim (Num U32)" in val.rename_monoexpr_correct(1)
       [OF _ val_proc_env_matches_\<xi>m_\<Xi> value_sem_rename_mono_prog_rename_\<Xi>_\<xi>m_\<xi>p]; clarsimp?)
-     apply (clarsimp simp: abbreviatedType1_def)
-     apply (clarsimp simp: val.matches_Cons[where xs = "[]" and ys = "[]", simplified])
-     apply (clarsimp simp: val.matches_def)
-     apply (rule val.v_t_record; simp?)
-     apply (rule val.v_t_r_cons1; clarsimp?)
-      apply (rule val.v_t_prim'; clarsimp)
-     apply (rule val.v_t_r_cons1; clarsimp?)
-      apply (rule val.v_t_prim'; clarsimp)
-     apply (rule val.v_t_r_cons1; clarsimp?)
-      apply (rule val.v_t_unit)
-     apply (rule val.v_t_r_empty)
-    apply (case_tac va; clarsimp)
-   apply (subst val_wa_foldnb_bod_0p.simps; clarsimp)
+      apply (clarsimp simp: abbreviatedType1_def)
+      apply (clarsimp simp: val.matches_Cons[where xs = "[]" and ys = "[]", simplified])
+      apply (clarsimp simp: val.matches_def)
+      apply (rule val.v_t_record; simp?)
+      apply (rule val.v_t_r_cons1; clarsimp?)
+       apply (erule_tac x = frm in allE; clarsimp)
+       apply (rule val.v_t_prim'; clarsimp)
+      apply (rule val.v_t_r_cons1; clarsimp?)
+       apply (rule val.v_t_prim'; clarsimp)
+      apply (rule val.v_t_r_cons1; clarsimp?)
+       apply (rule val.v_t_unit)
+      apply (rule val.v_t_r_empty)
+     apply (erule_tac x = frm in allE; clarsimp)
+    apply (case_tac v; clarsimp)
+   apply (subst val_wa_foldnb_bod_0.simps; clarsimp)
   apply (clarsimp simp: not_le)
   apply (frule_tac x = to in spec)
   apply (erule impE, simp)
@@ -504,11 +533,14 @@ lemma val_wa_foldnb_0_mono_helper2:
      apply (rule val.v_t_unit)
     apply (rule val.v_t_r_empty)
    apply (case_tac va; clarsimp)
-   apply (drule_tac v = v and r' = "VPrim (LU32 r)" in val_wa_foldnb_bod_0p_step; simp)
+   apply (drule_tac r' = "VPrim (LU32 r)" in val_wa_foldnb_bod_0_step; simp)
   apply (insert val_proc_env_matches_\<xi>m_\<Xi>)
   apply (clarsimp simp: abbreviatedType1_def)
   apply (drule val_wa_foldnb_bod_0_preservation; simp?)
-    apply (rule val.v_t_prim[where l = "LU32 _", simplified])
+     apply clarsimp
+     apply (erule_tac x = i in allE; clarsimp)
+     apply (rule val.v_t_prim'; clarsimp)
+    apply (rule val.v_t_prim'; clarsimp)
    apply (rule val.v_t_unit)
   apply (erule v_t_prim_tE)
   apply (drule lit_type_ex_32[OF sym])
@@ -516,7 +548,7 @@ lemma val_wa_foldnb_0_mono_helper2:
   done
 
 lemma value_sem_rename_mono_prog_rename_\<Xi>_\<xi>m1_\<xi>p1: 
-  "value_sem.rename_mono_prog abs_typing_v rename \<Xi> \<xi>m1 \<xi>p1"
+  "value_sem.rename_mono_prog wa_abs_typing_v rename \<Xi> \<xi>m1 \<xi>p1"
   apply (clarsimp simp: val.rename_mono_prog_def)
   apply (rule conjI; clarsimp)
    apply (rule_tac x = v' in exI)
@@ -567,7 +599,7 @@ lemma val_proc_env_matches_\<xi>m1_\<Xi>:
      apply (clarsimp simp: wordarray_get_0_type_def abbreviatedType3_def val_wa_get_def)
      apply (erule val.v_t_recordE)
      apply (erule val.v_t_r_consE; clarsimp)
-     apply (erule val.v_t_abstractE; clarsimp simp: abs_typing_v_def)
+     apply (erule val.v_t_abstractE; clarsimp simp: wa_abs_typing_v_def)
      apply (case_tac va; clarsimp)
     apply (rule val.v_t_prim[where l = "(LU32 _)", simplified])
    apply (clarsimp simp: wordarray_length_0_type_def val_wa_length_def)
@@ -577,12 +609,10 @@ lemma val_proc_env_matches_\<xi>m1_\<Xi>:
   apply (erule val.v_t_r_consE; clarsimp)
   apply (erule val.v_t_abstractE)
   apply (rule val.v_t_abstract; clarsimp)
-   apply (clarsimp simp: abs_typing_v_def)
+   apply (clarsimp simp: wa_abs_typing_v_def)
    apply (case_tac val; clarsimp)
    apply (erule_tac x = i in allE; clarsimp)
-   apply (case_tac "i = unat idx")
-    apply (rule_tac x = x4 in exI; simp)
-   apply (rule_tac x = x in exI; simp)
+   apply (case_tac "i = unat idx"; clarsimp)
   apply (clarsimp simp: wordarray_fold_no_break_0_type_def val_wa_foldnb_0_def)
   apply (erule val.v_t_recordE)
   apply (erule val.v_t_r_consE; clarsimp)+
@@ -590,9 +620,9 @@ lemma val_proc_env_matches_\<xi>m1_\<Xi>:
   done
 
 lemma upd_wa_foldnb_bod_0_pres_obsv:
-  "\<lbrakk>upd_wa_foldnb_bod_0 \<sigma> p frm to f acc (obsv, s) (\<sigma>', res); upd_val_rel \<Xi> \<sigma> obsv obsv' t s {};
-    \<sigma> p = option.Some (UAbstract (WAU32 len arr)); \<forall>i < len. \<exists>x. \<sigma> (arr + 4 * i) = option.Some (UPrim (LU32 x))\<rbrakk> 
-    \<Longrightarrow> upd_val_rel \<Xi> \<sigma>' obsv obsv' t s {}"
+  "\<lbrakk>upd_wa_foldnb_bod_0 \<xi>\<^sub>u \<sigma> p frm to f acc (obsv, s) (\<sigma>', res); upd_val_rel \<Xi>' \<sigma> obsv obsv' t s {};
+    \<sigma> p = option.Some (UAbstract (UWA (TPrim (Num n)) len arr)); \<forall>i < len. \<exists>x. \<sigma> (arr + size_of_num_type n * i) = option.Some x\<rbrakk> 
+    \<Longrightarrow> upd_val_rel \<Xi>' \<sigma>' obsv obsv' t s {}"
   apply (induct to arbitrary: \<sigma>' res)
    apply (erule upd_wa_foldnb_bod_0.elims; clarsimp)
   apply (case_tac "len < 1 + to")
@@ -607,7 +637,7 @@ lemma upd_wa_foldnb_bod_0_pres_obsv:
    apply clarsimp
    apply (drule_tac x = \<sigma>'' in meta_spec)
    apply (drule_tac x = r'' in meta_spec)
-   apply clarsimp thm upd_val_rel_frame
+   apply clarsimp
    apply (drule_tac upd_val_rel_frame(1); simp?)
    apply blast
   apply (case_tac "\<not> frm < 1 + to")
@@ -621,14 +651,14 @@ lemma upd_wa_foldnb_bod_0_pres_obsv:
   by (metis add.commute inc_le not_less word_le_less_eq)
 
 lemma upd_val_wa_foldnb_bod_0_corres:
-  "\<lbrakk>upd_wa_foldnb_bod_0 \<sigma> p frm to f acc (obsv, s) (\<sigma>', res); 
-    val_wa_foldnb_bod_0 xs (unat frm) (unat to) f acc' obsv' res';
-    \<sigma> p = option.Some (UAbstract (WAU32 len arr));
-    abs_upd_val' (WAU32 len arr) (VWA (TPrim (Num U32)) xs) ''WordArray'' [TPrim (Num U32)] (Boxed ReadOnly undefined) r w \<sigma>;
-    upd_val_rel \<Xi> \<sigma> acc acc' u ra wa; upd_val_rel \<Xi> \<sigma> obsv obsv' t s {}; wa \<inter> s = {}; proc_ctx_wellformed \<Xi>;
-    \<tau> = TRecord [(''elem'', (TPrim (Num U32), Present)), (''acc'', (u, Present)), (''obsv'', (t, Present))] Unboxed;
-    proc_env_u_v_matches \<xi>0 \<xi>m \<Xi>;  \<Xi>, [], [option.Some \<tau>] \<turnstile> App f (Var 0) : u\<rbrakk>
-    \<Longrightarrow> \<exists>ra' wa'.  upd_val_rel \<Xi> \<sigma>' res res' u ra' wa' \<and> ra' \<subseteq> ({p} \<union> ra \<union> s \<union> r)\<and> frame \<sigma> wa \<sigma>' wa'"
+  "\<lbrakk>upd_wa_foldnb_bod_0 \<xi>\<^sub>u \<sigma> p frm to f acc (obsv, s) (\<sigma>', res); 
+    val_wa_foldnb_bod_0 \<xi>\<^sub>v xs (unat frm) (unat to) f acc' obsv' res';
+    \<sigma> p = option.Some (UAbstract (UWA v len arr));
+    wa_abs_upd_val (UWA v len arr) (VWA v xs) ''WordArray'' [v] (Boxed ReadOnly undefined) r w \<sigma>;
+    upd_val_rel \<Xi>' \<sigma> acc acc' u ra wa; upd_val_rel \<Xi>' \<sigma> obsv obsv' t s {}; wa \<inter> s = {}; proc_ctx_wellformed \<Xi>';
+    \<tau> = TRecord [(''elem'', (v, Present)), (''acc'', (u, Present)), (''obsv'', (t, Present))] Unboxed;
+    proc_env_u_v_matches \<xi>\<^sub>u \<xi>\<^sub>v \<Xi>';  \<Xi>', [], [option.Some \<tau>] \<turnstile> App f (Var 0) : u\<rbrakk>
+    \<Longrightarrow> \<exists>ra' wa'.  upd_val_rel \<Xi>' \<sigma>' res res' u ra' wa' \<and> ra' \<subseteq> ({p} \<union> ra \<union> s \<union> r)\<and> frame \<sigma> wa \<sigma>' wa'"
   apply (induct to arbitrary: res res' \<sigma>')
    apply (erule upd_wa_foldnb_bod_0.elims; clarsimp)
    apply (erule val_wa_foldnb_bod_0.elims; clarsimp)
@@ -638,7 +668,9 @@ lemma upd_val_wa_foldnb_bod_0_corres:
   apply (case_tac "len < 1 + to")
    apply (drule upd_wa_foldnb_bod_0_back_step'; simp?)
    apply (drule unatSuc; clarsimp)
-   apply (drule val_wa_foldnb_bod_0_back_step'; clarsimp simp: abs_upd_val'_def word_less_nat_alt)
+   apply (drule val_wa_foldnb_bod_0_back_step'; clarsimp simp: wa_abs_upd_val_def word_less_nat_alt)
+   apply (case_tac v; clarsimp)
+   apply (case_tac x5; clarsimp)
   apply (case_tac "1 + to \<le> frm")
    apply (frule_tac y = "1 + to" and x = frm in leD)
    apply (erule upd_wa_foldnb_bod_0.elims; clarsimp)
@@ -650,64 +682,98 @@ lemma upd_val_wa_foldnb_bod_0_corres:
   apply (case_tac "frm = to")
    apply (clarsimp simp: not_le not_less)
    apply (erule upd_wa_foldnb_bod_0.elims; clarsimp split: if_split_asm)
+   apply (erule disjE; clarsimp)
     apply (erule upd_wa_foldnb_bod_0.elims; clarsimp simp: add.commute)
-    apply (drule unatSuc; clarsimp simp: word_less_nat_alt word_le_nat_alt abs_upd_val'_def)
+    apply (drule unatSuc; clarsimp simp: word_less_nat_alt word_le_nat_alt wa_abs_upd_val_def)
+    apply (case_tac v; clarsimp)
     apply (erule val_wa_foldnb_bod_0.elims; clarsimp)
     apply (erule val_wa_foldnb_bod_0.elims; clarsimp)
     apply (erule_tac x = frm in allE; clarsimp)
-    apply (frule_tac \<gamma> = "[URecord [(UPrim (LU32 v), RPrim (Num U32)), (acc, upd.uval_repr acc),
+    apply (frule_tac \<gamma> = "[URecord [(va, upd.uval_repr va), (acc, upd.uval_repr acc),
       (obsv, upd.uval_repr obsv)]]" and 
-      \<gamma>' = "[VRecord [VPrim (LU32 v), acc', obsv']]" and
+      \<gamma>' = "[VRecord [xs ! unat frm, acc', obsv']]" and
       r = "ra \<union> s" and w = wa in mono_correspondence(1); simp?)
      apply (rule u_v_matches_some[where r' = "{}" and w' = "{}", simplified])
       apply (rule u_v_struct; simp?)
       apply (rule u_v_r_cons1[where r = "{}" and w = "{}", simplified]; simp?)
-       apply (rule u_v_prim[where l = "LU32 _", simplified])
-      apply (rule u_v_r_cons1[where r = ra and w' = "{}", simplified]; simp?)
-       apply (rule u_v_r_cons1[where r' = "{}" and w' = "{}", simplified]; simp?)
-        apply (rule u_v_r_empty)
-       apply (drule_tac u = obsv in upd_val_rel_to_uval_typing(1))
+        apply (clarsimp simp: wa_abs_typing_v_def)
+        apply (erule_tac x = frm in allE; clarsimp)+
+        apply (erule_tac x = "unat frm" in allE; clarsimp)
+        apply (rule u_v_prim'; clarsimp)
+       apply (rule u_v_r_cons1[where r = ra and w' = "{}", simplified]; simp?)
+        apply (rule u_v_r_cons1[where r' = "{}" and w' = "{}", simplified]; simp?)
+         apply (rule u_v_r_empty)
+        apply (drule_tac u = obsv in upd_val_rel_to_uval_typing(1))
+        apply (drule upd.type_repr_uval_repr(1); simp)
+       apply (drule upd_val_rel_to_uval_typing(1))
        apply (drule upd.type_repr_uval_repr(1); simp)
-      apply (drule  upd_val_rel_to_uval_typing(1))
-      apply (drule upd.type_repr_uval_repr(1); simp)
+      apply (erule_tac x = frm in allE; clarsimp)+
      apply (rule u_v_matches_empty[where \<tau>s = "[]", simplified])
     apply clarsimp
     apply (rule_tac x = r' in exI)
     apply (rule_tac x = w' in exI; simp)
     apply blast
-   apply (rule FalseE)
-   apply (drule unatSuc; clarsimp simp: word_less_nat_alt word_le_nat_alt)
-  apply clarsimp
-  apply (subgoal_tac "\<exists>v. \<sigma> (arr + 4 * to) = option.Some (UPrim (LU32 v))")
+   apply (erule impE)
+    apply auto[1]
    apply clarsimp
-   apply (drule upd_wa_foldnb_bod_0_back_step; simp?)
-     apply (drule unatSuc; clarsimp simp: word_less_nat_alt)
-    apply (metis add.commute inc_le not_less_iff_gr_or_eq)
-   apply clarsimp
-   apply (drule unatSuc; clarsimp simp: word_less_nat_alt word_le_nat_alt)
-   apply (drule_tac v = v in val_wa_foldnb_bod_0_back_step; simp?)
-      apply (clarsimp simp: abs_upd_val'_def)
-     apply (meson Suc_leI not_less_iff_gr_or_eq word_less_nat_alt)
-    apply (clarsimp simp: abs_upd_val'_def)
-    apply (erule_tac x = to in allE; clarsimp)
-    apply (clarsimp simp: not_less word_less_nat_alt)
-   apply clarsimp
-   apply (drule_tac x = r'' in meta_spec)
-   apply (drule_tac x = r' in meta_spec)
-   apply (drule_tac x = \<sigma>'' in meta_spec)
-   apply clarsimp
-   apply (frule_tac \<gamma> = "[URecord [(UPrim (LU32 v), RPrim (Num U32)), (r'', upd.uval_repr r''), 
+   apply (erule upd_wa_foldnb_bod_0.elims; clarsimp simp: add.commute)
+    apply (drule unatSuc; clarsimp simp: word_less_nat_alt word_le_nat_alt wa_abs_upd_val_def)
+   apply (erule val_wa_foldnb_bod_0.elims; clarsimp)+
+   apply (frule_tac \<gamma> = "[URecord [(va, upd.uval_repr va), (acc, upd.uval_repr acc),
       (obsv, upd.uval_repr obsv)]]" and 
-      \<gamma>' = "[VRecord [VPrim (LU32 v), r', obsv']]" and
-      r = "ra' \<union> s" and w = wa' in mono_correspondence(1); simp?)
+      \<gamma>' = "[VRecord [xs ! unat frm, acc', obsv']]" and
+      r = "ra \<union> s" and w = wa in mono_correspondence(1); simp?)
     apply (rule u_v_matches_some[where r' = "{}" and w' = "{}", simplified])
-     apply (rule u_v_struct; simp?)
+      apply (rule u_v_struct; simp?)
      apply (rule u_v_r_cons1[where r = "{}" and w = "{}", simplified]; simp?)
-      apply (rule u_v_prim[where l = "LU32 _", simplified])
+       apply (clarsimp simp: wa_abs_typing_v_def)
+       apply (erule_tac x = frm in allE; clarsimp)+
+       apply (erule_tac x = "unat frm" in allE; clarsimp)
+       apply (rule u_v_prim'; clarsimp)
+      apply (rule u_v_r_cons1[where r = ra and w' = "{}", simplified]; simp?)
+       apply (rule u_v_r_cons1[where r' = "{}" and w' = "{}", simplified]; simp?)
+        apply (rule u_v_r_empty)
+       apply (drule_tac u = obsv in upd_val_rel_to_uval_typing(1))
+       apply (drule upd.type_repr_uval_repr(1); simp)
+      apply (drule upd_val_rel_to_uval_typing(1))
+      apply (drule upd.type_repr_uval_repr(1); simp)
+     apply (erule_tac x = frm in allE; clarsimp)+
+    apply (rule u_v_matches_empty[where \<tau>s = "[]", simplified])
+   apply clarsimp
+   apply (rule_tac x = r' in exI)
+   apply (rule_tac x = w' in exI)
+   apply clarsimp
+   apply blast
+  apply (clarsimp simp: wa_abs_upd_val_def)
+  apply (case_tac v; clarsimp)
+  apply (case_tac x5; clarsimp)
+  apply (drule upd_wa_foldnb_bod_0_back_step; simp?)
+    apply (drule unatSuc; clarsimp simp: word_less_nat_alt)
+   apply (metis add.commute inc_le not_less_iff_gr_or_eq)
+  apply (drule unatSuc; clarsimp simp: word_less_nat_alt word_le_nat_alt)
+  apply (drule_tac val_wa_foldnb_bod_0_back_step; simp?)
+   apply (meson Suc_leI not_less_iff_gr_or_eq word_less_nat_alt)
+  apply clarsimp
+  apply (drule_tac x = r'' in meta_spec)
+  apply (drule_tac x = r' in meta_spec)
+  apply (drule_tac x = \<sigma>'' in meta_spec)
+  apply clarsimp
+  apply (frule_tac \<gamma> = "[URecord [(va, upd.uval_repr va), (r'', upd.uval_repr r''),
+      (obsv, upd.uval_repr obsv)]]" and 
+      \<gamma>' = "[VRecord [xs ! unat to, r', obsv']]" and
+      r = "ra' \<union> s" and w = wa' in mono_correspondence(1); simp?)
+   apply (rule u_v_matches_some[where r' = "{}" and w' = "{}", simplified])
+    apply (rule u_v_struct; simp?)
+    apply (rule u_v_r_cons1[where r = "{}" and w = "{}", simplified]; simp?)
+      apply (erule_tac x = to in allE)
+      apply (clarsimp simp: not_less word_less_nat_alt)
+      apply (rule u_v_prim'; clarsimp)
      apply (rule u_v_r_cons1[where r' = s and w' = "{}", simplified]; simp?)
        apply (rule u_v_r_cons1[where r' = "{}" and w' = "{}", simplified]; simp?)
          apply (drule upd_wa_foldnb_bod_0_pres_obsv; simp?)
-         apply (clarsimp simp: abs_upd_val'_def abs_typing_u_def)
+         apply clarsimp
+         apply (erule_tac x = i in allE)
+         apply (clarsimp simp: word_less_nat_alt)
         apply (rule u_v_r_empty)
        apply (drule_tac u = obsv in upd_val_rel_to_uval_typing(1))
        apply (drule upd.type_repr_uval_repr(1); simp)
@@ -715,8 +781,9 @@ lemma upd_val_wa_foldnb_bod_0_corres:
       apply (thin_tac "frame _ _ _ _")
       apply (case_tac "\<exists>e. e \<in> wa' \<inter> s"; simp)
        apply (clarsimp simp: frame_def)
-       apply (erule_tac x = e in allE)
+       apply (erule_tac x = e in allE)+
        apply clarsimp
+       apply (thin_tac "_ \<longrightarrow> _")
        apply (erule impE)
         apply (drule_tac x = e in orthD2; simp)
        apply (drule upd_val_rel_to_uval_typing(1))
@@ -724,28 +791,26 @@ lemma upd_val_wa_foldnb_bod_0_corres:
       apply blast
      apply (drule_tac u = r'' in upd_val_rel_to_uval_typing(1))
      apply (drule upd.type_repr_uval_repr(1); simp)
-    apply (rule u_v_matches_empty[where \<tau>s = "[]", simplified])
-   apply clarsimp
-   apply (rule_tac x = r'a in exI)
-   apply (rule_tac x = w' in exI)
-   apply clarsimp
-   apply (rule conjI)
-    apply blast
-   apply (rule upd.frame_trans; simp)
-  apply (clarsimp simp: abs_upd_val'_def)
-  apply (erule_tac x = to in allE)
-  apply (erule impE)
-   apply (drule unatSuc; clarsimp simp: word_less_nat_alt)
+    apply (erule_tac x = to in allE; clarsimp)
+   apply (rule u_v_matches_empty[where \<tau>s = "[]", simplified])
   apply clarsimp
+  apply (rule_tac x = r'a in exI)
+  apply (rule_tac x = w' in exI)
+  apply clarsimp
+  apply (rule conjI)
+   apply blast
+  apply (rule upd.frame_trans; simp)
   done
 
+
+
 lemma val_executes_from_upd_wa_foldnb_bod_0:
-  "\<lbrakk>upd_wa_foldnb_bod_0 \<sigma> p frm to f acc (obsv, s) (\<sigma>', res); \<sigma> p = option.Some (UAbstract (WAU32 len arr));
-    abs_upd_val' (WAU32 len arr) (VWA (TPrim (Num U32)) xs) ''WordArray'' [TPrim (Num U32)] (Boxed ReadOnly undefined) r w \<sigma>;
-    upd_val_rel \<Xi> \<sigma> acc acc' u ra wa; upd_val_rel \<Xi> \<sigma> obsv obsv' t s {}; wa \<inter> s = {}; proc_ctx_wellformed \<Xi>;
-    \<tau> = TRecord [(''elem'', (TPrim (Num U32), Present)), (''acc'', (u, Present)), (''obsv'', (t, Present))] Unboxed;
-    proc_env_u_v_matches \<xi>0 \<xi>m \<Xi>;  \<Xi>, [], [option.Some \<tau>] \<turnstile> App f (Var 0) : u\<rbrakk>
-    \<Longrightarrow> \<exists>res' r w. val_wa_foldnb_bod_0 xs (unat frm) (unat to) f acc' obsv' res' \<and> upd_val_rel \<Xi> \<sigma>' res res' u r w"
+  "\<lbrakk>upd_wa_foldnb_bod_0 \<xi>\<^sub>u \<sigma> p frm to f acc (obsv, s) (\<sigma>', res); \<sigma> p = option.Some (UAbstract (UWA v len arr));
+    wa_abs_upd_val (UWA v len arr) (VWA v xs) ''WordArray'' [v] (Boxed ReadOnly undefined) r w \<sigma>;
+    upd_val_rel \<Xi>' \<sigma> acc acc' u ra wa; upd_val_rel \<Xi>' \<sigma> obsv obsv' t s {}; wa \<inter> s = {}; proc_ctx_wellformed \<Xi>';
+    \<tau> = TRecord [(''elem'', (v, Present)), (''acc'', (u, Present)), (''obsv'', (t, Present))] Unboxed;
+    proc_env_u_v_matches \<xi>\<^sub>u \<xi>\<^sub>v \<Xi>';  \<Xi>', [], [option.Some \<tau>] \<turnstile> App f (Var 0) : u\<rbrakk>
+    \<Longrightarrow> \<exists>res' r w. val_wa_foldnb_bod_0 \<xi>\<^sub>v xs (unat frm) (unat to) f acc' obsv' res' \<and> upd_val_rel \<Xi>' \<sigma>' res res' u r w"
   apply (induct arbitrary: \<sigma>' res rule: word_induct[where m = "to"])
    apply (erule upd_wa_foldnb_bod_0.elims; clarsimp)
    apply (rule_tac x = acc' in exI)
@@ -767,12 +832,16 @@ lemma val_executes_from_upd_wa_foldnb_bod_0:
    apply clarsimp
    apply (rule_tac x = res' in exI)
    apply (drule val_wa_foldnb_bod_0_to_geq_lenD)
-    apply (clarsimp simp: abs_upd_val'_def)
+    apply (clarsimp simp: wa_abs_upd_val_def)
+    apply (case_tac v; clarsimp)
+    apply (case_tac x5; clarsimp)
     apply (simp add: unatSuc word_less_nat_alt)
    apply (drule unatSuc; clarsimp)
    apply (rule conjI)
     apply (rule val_wa_foldnb_bod_0_to_geq_len; simp?)
-    apply (clarsimp simp: abs_upd_val'_def word_less_nat_alt)
+    apply (clarsimp simp: wa_abs_upd_val_def)
+    apply (case_tac v; clarsimp)
+    apply (case_tac x5; clarsimp simp: word_less_nat_alt)
    apply (rule_tac x = rb in exI)
    apply (rule_tac x = x in exI)
    apply clarsimp
@@ -788,130 +857,191 @@ lemma val_executes_from_upd_wa_foldnb_bod_0:
   apply (case_tac "frm = n")
    apply (clarsimp simp: not_le not_less)
    apply (erule upd_wa_foldnb_bod_0.elims; clarsimp split: if_split_asm)
+   apply (erule disjE; clarsimp)
     apply (erule upd_wa_foldnb_bod_0.elims; clarsimp simp: add.commute)
-    apply (frule_tac \<gamma> = "[URecord [(UPrim (LU32 v), RPrim (Num U32)), (acc, upd.uval_repr acc), 
+    apply (frule_tac \<gamma> = "[URecord [(va, upd.uval_repr va), (acc, upd.uval_repr acc), 
       (obsv, upd.uval_repr obsv)]]" and 
-      \<gamma>' = "[VRecord [VPrim (LU32 v), acc', obsv']]" and
+      \<gamma>' = "[VRecord [xs ! unat frm, acc', obsv']]" and
       r = "ra \<union> s" and w = wa in val_executes_from_upd_executes(1); simp?)
      apply (rule u_v_matches_some[where r' = "{}" and w' = "{}", simplified])
       apply (rule u_v_struct; simp?)
       apply (rule u_v_r_cons1[where r = "{}" and w = "{}", simplified]; simp?)
-       apply (rule u_v_prim[where l = "LU32 _", simplified])
-      apply (rule u_v_r_cons1[where r' = s and w' = "{}", simplified]; simp?)
-       apply (rule u_v_r_cons1[where r' = "{}" and w' = "{}", simplified]; simp?)
-        apply (rule u_v_r_empty)
-       apply (drule_tac u = obsv in  upd_val_rel_to_uval_typing(1))
+        apply (clarsimp simp: wa_abs_upd_val_def)
+        apply (erule_tac x = frm in allE; clarsimp)+
+        apply (rule u_v_prim'; clarsimp)
+       apply (rule u_v_r_cons1[where r' = s and w' = "{}", simplified]; simp?)
+        apply (rule u_v_r_cons1[where r' = "{}" and w' = "{}", simplified]; simp?)
+         apply (rule u_v_r_empty)
+        apply (drule_tac u = obsv in upd_val_rel_to_uval_typing(1))
+        apply (drule upd.type_repr_uval_repr(1); simp)
+       apply (drule upd_val_rel_to_uval_typing(1))
        apply (drule upd.type_repr_uval_repr(1); simp)
-      apply (drule upd_val_rel_to_uval_typing(1))
-      apply (drule upd.type_repr_uval_repr(1); simp)
+      apply (clarsimp simp: wa_abs_upd_val_def)
+      apply (erule_tac x = frm in allE; clarsimp)+
      apply (rule u_v_matches_empty[where \<tau>s = "[]", simplified])
     apply clarsimp
     apply (rule_tac x = v' in exI)
+    apply (drule unatSuc; clarsimp simp: word_less_nat_alt word_le_nat_alt)
     apply (rule conjI)
-     apply (clarsimp simp: abs_upd_val'_def)
-     apply (erule_tac x = frm in allE; clarsimp)
-     apply (drule unatSuc; clarsimp simp: word_less_nat_alt word_le_nat_alt)
      apply (subst val_wa_foldnb_bod_0.simps; clarsimp)
      apply (subst val_wa_foldnb_bod_0.simps; clarsimp)
-    apply (frule_tac \<gamma> = "[URecord [(UPrim (LU32 v), RPrim (Num U32)), (acc, upd.uval_repr acc),
+     apply (rule FalseE)
+     apply (clarsimp simp: wa_abs_upd_val_def)
+    apply (frule_tac \<gamma> = "[URecord [(va, upd.uval_repr va), (acc, upd.uval_repr acc),
       (obsv, upd.uval_repr obsv)]]" and 
-      \<gamma>' = "[VRecord [VPrim (LU32 v), acc', obsv']]" and
+      \<gamma>' = "[VRecord [xs ! unat frm, acc', obsv']]" and
       r = "ra \<union> s" and w = wa in mono_correspondence(1); simp?)
      apply (rule u_v_matches_some[where r' = "{}" and w' = "{}", simplified])
       apply (rule u_v_struct; simp?)
       apply (rule u_v_r_cons1[where r = "{}" and w = "{}", simplified]; simp?)
-       apply (rule u_v_prim[where l = "LU32 _", simplified])
-      apply (rule u_v_r_cons1[where r' = s and w' = "{}", simplified]; simp?)
-       apply (rule u_v_r_cons1[where r' = "{}" and w' = "{}", simplified]; simp?)
-        apply (rule u_v_r_empty)
-       apply (drule_tac u = obsv in  upd_val_rel_to_uval_typing(1))
+        apply (clarsimp simp: wa_abs_upd_val_def)
+        apply (erule_tac x = frm in allE; clarsimp simp: word_less_nat_alt)+
+        apply (rule u_v_prim'; clarsimp)
+       apply (rule u_v_r_cons1[where r' = s and w' = "{}", simplified]; simp?)
+        apply (rule u_v_r_cons1[where r' = "{}" and w' = "{}", simplified]; simp?)
+         apply (rule u_v_r_empty)
+        apply (drule_tac u = obsv in  upd_val_rel_to_uval_typing(1))
+        apply (drule upd.type_repr_uval_repr(1); simp)
+       apply (drule upd_val_rel_to_uval_typing(1))
        apply (drule upd.type_repr_uval_repr(1); simp)
-      apply (drule upd_val_rel_to_uval_typing(1))
-      apply (drule upd.type_repr_uval_repr(1); simp)
+      apply (clarsimp simp: wa_abs_upd_val_def)
+      apply (erule_tac x = frm in allE; clarsimp simp: word_less_nat_alt)+
      apply (rule u_v_matches_empty[where \<tau>s = "[]", simplified])
     apply clarsimp
     apply (rule_tac x = r' in exI)
     apply (rule_tac x = w' in exI)
     apply clarsimp
-   apply (rule FalseE)
-   apply simp
-  apply (subgoal_tac "\<exists>v. \<sigma> (arr + 4 * n) = option.Some (UPrim (LU32 v))")
+   apply (erule impE)
+    apply simp
    apply clarsimp
-   apply (drule_tac v = v in upd_wa_foldnb_bod_0_back_step; simp?)
-     apply (metis word_le_less_eq word_zero_le)
-    apply (metis add.commute plus_one_helper word_le_less_eq word_not_le)
+   apply (erule upd_wa_foldnb_bod_0.elims; clarsimp simp: add.commute)
+   apply (drule unatSuc; clarsimp simp: word_less_nat_alt word_le_nat_alt)
+   apply (frule_tac \<gamma> = "[URecord [(va, upd.uval_repr va), (acc, upd.uval_repr acc), 
+      (obsv, upd.uval_repr obsv)]]" and
+      \<gamma>' = "[VRecord [xs ! unat frm, acc', obsv']]" and
+      r = "ra \<union> s" and w = wa in val_executes_from_upd_executes(1); simp?)
+    apply (rule u_v_matches_some[where r' = "{}" and w' = "{}", simplified])
+  apply (rule u_v_struct; simp?)
+     apply (rule u_v_r_cons1[where r = "{}" and w = "{}", simplified]; simp?)
+       apply (clarsimp simp: wa_abs_upd_val_def)
+       apply (erule_tac x = frm in allE; clarsimp simp: word_less_nat_alt)+
+       apply (rule u_v_prim'; clarsimp)
+      apply (rule u_v_r_cons1[where r' = s and w' = "{}", simplified]; simp?)
+       apply (rule u_v_r_cons1[where r' = "{}" and w' = "{}", simplified]; simp?)
+        apply (rule u_v_r_empty)
+       apply (drule_tac u = obsv in upd_val_rel_to_uval_typing(1))
+       apply (drule upd.type_repr_uval_repr(1); simp)
+      apply (drule upd_val_rel_to_uval_typing(1))
+      apply (drule upd.type_repr_uval_repr(1); simp)
+     apply (clarsimp simp: wa_abs_upd_val_def)
+     apply (erule_tac x = frm in allE; clarsimp simp: word_less_nat_alt)+
+    apply (rule u_v_matches_empty[where \<tau>s = "[]", simplified])
+   apply clarsimp
+   apply (frule_tac \<gamma> = "[URecord [(va, upd.uval_repr va), (acc, upd.uval_repr acc),
+      (obsv, upd.uval_repr obsv)]]" and 
+      \<gamma>' = "[VRecord [xs ! unat frm, acc', obsv']]" and
+      r = "ra \<union> s" and w = wa in mono_correspondence(1); simp?)
+    apply (rule u_v_matches_some[where r' = "{}" and w' = "{}", simplified])
+     apply (rule u_v_struct; simp?)
+     apply (rule u_v_r_cons1[where r = "{}" and w = "{}", simplified]; simp?)
+       apply (clarsimp simp: wa_abs_upd_val_def)
+       apply (erule_tac x = frm in allE; clarsimp simp: word_less_nat_alt)+
+       apply (rule u_v_prim'; clarsimp)
+      apply (rule u_v_r_cons1[where r' = s and w' = "{}", simplified]; simp?)
+       apply (rule u_v_r_cons1[where r' = "{}" and w' = "{}", simplified]; simp?)
+        apply (rule u_v_r_empty)
+       apply (drule_tac u = obsv in upd_val_rel_to_uval_typing(1))
+       apply (drule upd.type_repr_uval_repr(1); simp)
+      apply (drule upd_val_rel_to_uval_typing(1))
+      apply (drule upd.type_repr_uval_repr(1); simp)
+     apply (clarsimp simp: wa_abs_upd_val_def)
+     apply (erule_tac x = frm in allE; clarsimp simp: word_less_nat_alt)+
+    apply (rule u_v_matches_empty[where \<tau>s = "[]", simplified])
+   apply clarsimp
+   apply (clarsimp simp: wa_abs_upd_val_def)
+   apply (rule_tac x = v' in exI)
+   apply (subst val_wa_foldnb_bod_0.simps; clarsimp)+
+   apply (rule_tac x = r' in exI)
+   apply (rule_tac x = w' in exI)
+   apply clarsimp
+  apply (clarsimp simp: wa_abs_upd_val_def)
+  apply (case_tac v; clarsimp)
+  apply (case_tac x5; clarsimp)
+  apply (drule_tac upd_wa_foldnb_bod_0_back_step; simp?)
+    apply (metis word_le_less_eq word_zero_le)
+   apply (metis add.commute plus_one_helper word_le_less_eq word_not_le)
    apply clarsimp
    apply (drule_tac x = \<sigma>'' in meta_spec)
    apply (drule_tac x = r'' in meta_spec)
    apply clarsimp
-   apply (frule upd_val_wa_foldnb_bod_0_corres; simp?)
+  apply (frule_tac r = r and w = w in upd_val_wa_foldnb_bod_0_corres; simp?)
+   apply (clarsimp simp: wa_abs_upd_val_def)
   apply clarsimp
-   apply (subgoal_tac "wa' \<inter> s = {}")
-    apply (frule_tac \<gamma> = "[URecord [(UPrim (LU32 v), RPrim (Num U32)), (r'', upd.uval_repr r''), 
-      (obsv, upd.uval_repr obsv)]]" and 
-      \<gamma>' = "[VRecord [VPrim (LU32 v), res', obsv']]" and
+  apply (drule unatSuc; clarsimp simp: word_less_nat_alt word_le_nat_alt)
+  apply (frule_tac \<gamma> = "[URecord [(va, upd.uval_repr va), (r'', upd.uval_repr r''), 
+      (obsv, upd.uval_repr obsv)]]" and
+      \<gamma>' = "[VRecord [xs ! unat n, res', obsv']]" and
       r = "ra' \<union> s" and w = wa' in val_executes_from_upd_executes(1); simp?)
-     apply (rule u_v_matches_some[where r' = "{}" and w' = "{}", simplified])
-      apply (rule u_v_struct; simp?)
-      apply (rule u_v_r_cons1[where r = "{}" and w = "{}", simplified]; simp?)
-       apply (rule u_v_prim[where l = "LU32 _", simplified])
-      apply (rule u_v_r_cons1[where r' = s and w' = "{}", simplified]; simp?)
+   apply (rule u_v_matches_some[where r' = "{}" and w' = "{}", simplified])
+    apply (rule u_v_struct; simp?)
+    apply (rule u_v_r_cons1[where r = "{}" and w = "{}", simplified]; simp?)
+      apply (erule_tac x = n in allE; clarsimp)+
+      apply (rule u_v_prim'; clarsimp)
+     apply (rule u_v_r_cons1[where r' = s and w' = "{}", simplified]; simp?)
        apply (rule u_v_r_cons1[where r' = "{}" and w' = "{}", simplified]; simp?)
          apply (drule upd_wa_foldnb_bod_0_pres_obsv; simp?)
-         apply (clarsimp simp: abs_upd_val'_def abs_typing_u_def)
+         apply clarsimp
+         apply (erule_tac x = i in allE; clarsimp simp: word_less_nat_alt)+
         apply (rule u_v_r_empty)
        apply (drule_tac u = obsv in  upd_val_rel_to_uval_typing(1))
        apply (drule upd.type_repr_uval_repr(1); simp)
-      apply (drule_tac u = r'' in  upd_val_rel_to_uval_typing(1))
-      apply (drule upd.type_repr_uval_repr(1); simp)
-     apply (rule u_v_matches_empty[where \<tau>s = "[]", simplified])
-    apply clarsimp
-    apply (drule unatSuc; clarsimp simp: word_less_nat_alt word_le_nat_alt)
-    apply (drule_tac val_wa_foldnb_bod_0_step; simp?)
-      apply (clarsimp simp: abs_upd_val'_def)
-     apply (clarsimp simp: abs_upd_val'_def word_less_nat_alt)
-     apply (erule_tac x = n in allE)
-     apply clarsimp
-    apply (rule_tac x = v' in exI)
-    apply clarsimp
-    apply (frule_tac \<gamma> = "[URecord [(UPrim (LU32 v), RPrim (Num U32)), (r'', upd.uval_repr r''), 
-      (obsv, upd.uval_repr obsv)]]" and 
-      \<gamma>' = "[VRecord [VPrim (LU32 v), res', obsv']]" and
-      r = "ra' \<union> s" and w = wa' in mono_correspondence(1); simp?)
-     apply (rule u_v_matches_some[where r' = "{}" and w' = "{}", simplified])
-      apply (rule u_v_struct; simp?)
-      apply (rule u_v_r_cons1[where r = "{}" and w = "{}", simplified]; simp?)
-       apply (rule u_v_prim[where l = "LU32 _", simplified])
-      apply (rule u_v_r_cons1[where r' = s and w' = "{}", simplified]; simp?)
-       apply (rule u_v_r_cons1[where r' = "{}" and w' = "{}", simplified]; simp?)
-         apply (drule upd_wa_foldnb_bod_0_pres_obsv; simp?)
-         apply (clarsimp simp: abs_upd_val'_def abs_typing_u_def)
-        apply (rule u_v_r_empty)
-       apply (drule_tac u = obsv in  upd_val_rel_to_uval_typing(1))
-       apply (drule upd.type_repr_uval_repr(1); simp)
-      apply (drule_tac u = r'' in  upd_val_rel_to_uval_typing(1))
-      apply (drule upd.type_repr_uval_repr(1); simp)
-     apply (rule u_v_matches_empty[where \<tau>s = "[]", simplified])
-    apply clarsimp
-    apply (rule_tac x = r' in exI)
-    apply (rule_tac x = w' in exI)
-    apply simp
-   apply (case_tac "\<exists>e. e \<in> wa' \<inter> s"; simp)
-    apply (thin_tac "frame _ _ _ _")
-    apply (thin_tac "upd_val_rel _ _ r'' _ _ _ _")
-    apply (clarsimp simp: frame_def)
-    apply (erule_tac x = e in allE)
-    apply clarsimp
-    apply (erule impE)
-     apply blast
-    apply (drule_tac u = obsv in upd_val_rel_to_uval_typing(1))
-    apply (drule_tac p = e in upd.uval_typing_valid(1)[rotated 1]; simp?)
-   apply blast
-  apply (clarsimp simp: abs_upd_val'_def)
-  apply (erule_tac x = n in allE)
-  apply (erule impE)
-   apply (metis add.commute plus_one_helper2 word_not_le)
+      apply (rule disjointI)
+      apply (thin_tac "frame _ _ _ _")
+      apply (clarsimp simp: frame_def)
+      apply (erule_tac x = y in allE; clarsimp)+
+      apply (drule_tac x = y in orthD2; simp)
+      apply (drule_tac u = obsv and p = y in upd_val_rel_valid(1)[where r = s and w = "{}", simplified]; simp?)
+      apply clarsimp
+     apply (drule_tac u = r'' in  upd_val_rel_to_uval_typing(1))
+     apply (drule upd.type_repr_uval_repr(1); simp)
+    apply (erule_tac x = n in allE; clarsimp)+
+   apply (rule u_v_matches_empty[where \<tau>s = "[]", simplified])
   apply clarsimp
+  apply (drule_tac r' = v' in  val_wa_foldnb_bod_0_step; simp?)
+  apply (rule_tac x = v' in exI)
+  apply clarsimp
+  apply (frule_tac \<gamma> = "[URecord [(va, upd.uval_repr va), (r'', upd.uval_repr r''), 
+      (obsv, upd.uval_repr obsv)]]" and 
+      \<gamma>' = "[VRecord [xs ! unat n, res', obsv']]" and
+      r = "ra' \<union> s" and w = wa' in mono_correspondence(1); simp?)
+   apply (rule u_v_matches_some[where r' = "{}" and w' = "{}", simplified])
+    apply (rule u_v_struct; simp?)
+    apply (rule u_v_r_cons1[where r = "{}" and w = "{}", simplified]; simp?)
+      apply (erule_tac x = n in allE; clarsimp)
+      apply (rule u_v_prim'; clarsimp)
+     apply (rule u_v_r_cons1[where r' = s and w' = "{}", simplified]; simp?)
+       apply (rule u_v_r_cons1[where r' = "{}" and w' = "{}", simplified]; simp?)
+         apply (drule upd_wa_foldnb_bod_0_pres_obsv; simp?)
+         apply clarsimp
+         apply (erule_tac x = i in allE; clarsimp simp: word_less_nat_alt)
+        apply (rule u_v_r_empty)
+       apply (drule_tac u = obsv in  upd_val_rel_to_uval_typing(1))
+       apply (drule upd.type_repr_uval_repr(1); simp)
+      apply (rule disjointI)
+      apply (thin_tac "frame _ _ _ _")
+      apply (clarsimp simp: frame_def)
+      apply (erule_tac x = y in allE; clarsimp)+
+      apply (drule_tac x = y in orthD2; simp)
+      apply (drule_tac u = obsv and p = y in upd_val_rel_valid(1)[where r = s and w = "{}", simplified]; simp?)
+      apply clarsimp
+     apply (drule_tac u = r'' in  upd_val_rel_to_uval_typing(1))
+     apply (drule upd.type_repr_uval_repr(1); simp)
+    apply (erule_tac x = n in allE; clarsimp)
+   apply (rule u_v_matches_empty[where \<tau>s = "[]", simplified])
+  apply clarsimp
+  apply (rule_tac x = r' in exI)
+  apply (rule_tac x = w' in exI)
+  apply simp
   done
 
 lemma wordarray_fold_no_break_upd_val:
@@ -977,10 +1107,9 @@ lemma wordarray_fold_no_break_upd_val:
   apply clarsimp
   apply (erule disjE; clarsimp?)
   apply (erule disjE; clarsimp?)
-  apply (case_tac a'; clarsimp simp: abs_upd_val'_def val_wa_foldnb_0_def)
+  apply (case_tac a'; clarsimp simp: wa_abs_upd_val_def val_wa_foldnb_0_def)
   apply (case_tac x11; clarsimp)
   apply (case_tac x5; clarsimp)
-  apply (case_tac x1; clarsimp)
   apply (case_tac x; clarsimp)
    apply (subst (asm) upd_val_rel.simps[of _ _ "UFunction _ _", simplified])
    apply clarsimp
@@ -988,19 +1117,18 @@ lemma wordarray_fold_no_break_upd_val:
    apply (erule disjE; clarsimp?)
    apply (rule conjI; clarsimp)
     apply (drule_tac xs = x12 and r = r and w = "{}" and acc' = "VPrim (LU32 acc)" and
-      ra = "{}" and wa = "{}" and obsv' = "VUnit" and t = "TUnit" 
+      ra = "{}" and wa = "{}" and obsv' = "VUnit" and t = "TUnit"
       in upd_val_wa_foldnb_bod_0_corres; simp?)
-         apply (clarsimp simp: abs_upd_val'_def)
+         apply (clarsimp simp: wa_abs_upd_val_def)
         apply (rule u_v_prim'; clarsimp)
        apply (rule u_v_unit)
       apply (rule proc_ctx_wellformed_\<Xi>)
      apply (clarsimp simp: abbreviatedType1_def)
     apply (rule proc_env_u_v_matches_\<xi>0_\<xi>m_\<Xi>)
-   apply (clarsimp simp: abs_typing_v_def)
    apply (drule_tac xs = x12 and r = r and w = "{}" and acc' = "VPrim (LU32 acc)" and
       ra = "{}" and wa = "{}" and obsv' = "VUnit" and t = "TUnit" 
       in val_executes_from_upd_wa_foldnb_bod_0; simp?)
-         apply (clarsimp simp: abs_upd_val'_def abs_typing_v_def)
+         apply (clarsimp simp: wa_abs_upd_val_def wa_abs_typing_v_def)
         apply (rule u_v_prim'; clarsimp)
        apply (rule u_v_unit)
       apply (rule proc_ctx_wellformed_\<Xi>)
@@ -1010,11 +1138,20 @@ lemma wordarray_fold_no_break_upd_val:
    apply (rule_tac x = res' in exI)
    apply (clarsimp simp: val_wa_foldnb_0_def)
    apply (clarsimp simp: abbreviatedType1_def)
-   apply (drule val_wa_foldnb_bod_0_preservation[OF proc_ctx_wellformed_\<Xi> val_proc_env_matches_\<xi>m_\<Xi>]; simp?)
+   apply (rule conjI)
+    apply (clarsimp simp: wa_abs_typing_v_def)
+   apply (rule conjI)
+    apply (drule val_wa_foldnb_bod_0_preservation[OF proc_ctx_wellformed_\<Xi> val_proc_env_matches_\<xi>m_\<Xi>]; simp?)
+       apply (clarsimp simp: wa_abs_typing_v_def)
+       apply (erule_tac x = i in allE; clarsimp)+
+      apply (rule val.v_t_prim'; simp)
      apply (rule val.v_t_prim'; simp)
     apply (rule val.v_t_unit)
    apply (erule v_t_prim_tE; clarsimp)
-   apply (drule lit_type_ex_32[OF sym]; simp)
+    apply (drule lit_type_ex_32[OF sym]; simp)
+   apply (clarsimp simp: wa_abs_typing_v_def)
+   apply (erule_tac x = i in allE; clarsimp)
+   apply (drule lit_type_ex_32; simp)
   apply (subst (asm) upd_val_rel.simps[of _ _ "UAFunction _ _", simplified])
   apply clarsimp
   apply (erule disjE; clarsimp?)
@@ -1023,7 +1160,7 @@ lemma wordarray_fold_no_break_upd_val:
    apply (drule_tac xs = x12 and r = r and w = "{}" and acc' = "VPrim (LU32 acc)" and
       ra = "{}" and wa = "{}" and obsv' = "VUnit" and t = "TUnit" 
       in upd_val_wa_foldnb_bod_0_corres; simp?)
-        apply (clarsimp simp: abs_upd_val'_def)
+        apply (clarsimp simp: wa_abs_upd_val_def)
        apply (rule u_v_prim'; clarsimp)
       apply (rule u_v_unit)
      apply (rule proc_ctx_wellformed_\<Xi>)
@@ -1032,7 +1169,7 @@ lemma wordarray_fold_no_break_upd_val:
   apply (drule_tac xs = x12 and r = r and w = "{}" and acc' = "VPrim (LU32 acc)" and
       ra = "{}" and wa = "{}" and obsv' = "VUnit" and t = "TUnit" 
       in val_executes_from_upd_wa_foldnb_bod_0; simp?)
-        apply (clarsimp simp: abs_upd_val'_def)
+        apply (clarsimp simp: wa_abs_upd_val_def wa_abs_typing_v_def)
        apply (rule u_v_prim'; clarsimp)
       apply (rule u_v_unit)
      apply (rule proc_ctx_wellformed_\<Xi>)
@@ -1040,13 +1177,19 @@ lemma wordarray_fold_no_break_upd_val:
    apply (rule proc_env_u_v_matches_\<xi>0_\<xi>m_\<Xi>)
   apply clarsimp
   apply (rule_tac x = res' in exI)
-  apply (clarsimp simp: val_wa_foldnb_0_def abs_typing_v_def)
+  apply (clarsimp simp: val_wa_foldnb_0_def wa_abs_typing_v_def)
   apply (clarsimp simp: abbreviatedType1_def)
   apply (drule val_wa_foldnb_bod_0_preservation[OF proc_ctx_wellformed_\<Xi> val_proc_env_matches_\<xi>m_\<Xi>]; simp?)
+     apply clarsimp
+     apply (erule_tac x = i in allE; clarsimp)+
+     apply (rule val.v_t_prim'; simp)
     apply (rule val.v_t_prim'; simp)
    apply (rule val.v_t_unit)
   apply (erule v_t_prim_tE; clarsimp)
   apply (drule lit_type_ex_32[OF sym]; simp)
+  apply clarsimp
+  apply (erule_tac x = i in allE; clarsimp)
+  apply (drule lit_type_ex_32; simp)
   done
 
 
